rocq-osiris/examples/proofs/fold_array.v
@@ -1,0 +1,152 @@
+From osiris Require Import osiris.
+From iris.proofmode Require Import ltac_tactics.
+
+From osiris.examples Require Import og_fold_array.
+From osiris.stdlib.proofs Require Import array.
+
+From Stdlib.Logic Require Import FunctionalExtensionality.
+
+Section verification.
+
+  Context `{!osirisGS Σ}.
+
+  Open Scope Z.
+
+  Definition sum_spec : Z → microvx → iProp Σ :=
+    λ n m,
+      (⌜0 ≤ n ≤ max_array⌝ -∗
+       imp m {{ λ i, ⌜i = n * (n + 1) / 2⌝ }})%I.
+
+  Definition esum := EAnonFun __fun2.
+
+  Lemma imp_EPath_spec {E : coPset} {Ψ : iEff Σ} {A : Type} {EncA : Encode A}
+  {Φ : A → iProp Σ} {ζ : exn → iProp Σ} (η : env) (p : path) :
+    lookup_spec η p Φ -∗ imp eval η (EPath p) @ E <| Ψ |> ⟨⟨ ζ ⟩⟩ {{ λ a, □ Φ a }}.
+  Proof.
+    iIntros "(% & %Hpath & #HΦ)".
+    simpl_eval.
+    iApply imp_widen. rewrite Hpath. iApply imp_ret; eauto.
+  Qed.
+
+  Lemma lookup_spec_step {A : Type} `{Encode A} {Φ : A → iProp Σ} {η x p} mspec :
+    lookup_spec η [x] mspec -∗
+    (∀ (δ : env), mspec δ -∗ lookup_spec δ p Φ) -∗
+    lookup_spec η (x :: p) Φ.
+  Proof.
+    iIntros "(%δ & %Hlookup & #Hpost) Hcov".
+    iDestruct ("Hcov" with "Hpost") as "(% & %Hlookup' & #HΦ)".
+    iFrame "#". iPureIntro.
+    simpl. destruct p.
+    - simpl in Hlookup'. discriminate Hlookup'.
+    - simpl in Hlookup.
+      rewrite Hlookup !bind_ret.
+      assumption.
+  Qed.
+
+  Lemma lookup_spec_search {A : Type} `{Encode A} {Φ : A → iProp Σ} {η v p} x y :
+    (x =? y)%string = false →
+    lookup_spec ((y, v) :: η) (x :: p) Φ =
+    lookup_spec η (x :: p) Φ.
+  Proof.
+    intros Hneq.
+    unfold lookup_spec. f_equal.
+    extensionality v'. f_equal. f_equal.
+    destruct p; simpl.
+    - unfold lookup_name. rewrite Hneq. reflexivity.
+    - unfold lookup_name. rewrite Hneq. reflexivity.
+  Qed.
+
+  Lemma imp_EPath_var {E Ψ ζ} {A : Type} `{Encode A} {η p} (a : A) :
+    lookup_path η p = ret #a →
+    ⊢ imp (eval η (EPath p)) @ E <|Ψ|> ⟨⟨ ζ ⟩⟩ {{ λ a', ⌜a' = a⌝ }}.
+  Proof.
+    iIntros (Hlookup).
+    iApply imp_EPath; eauto.
+  Qed.
+
+  Lemma lookup_spec_mono {A : Type} `{Encode A} {η p} (Φ Φ' : A → iProp Σ) :
+    lookup_spec η p Φ' -∗
+    □ (∀ a, Φ' a -∗ Φ a) -∗
+    lookup_spec η p Φ.
+  Proof.
+    iIntros "(%a & %Hlookup & #HΦ') #Hcov".
+    iExists a; iSplit; first (iPureIntro; assumption).
+    iIntros "!>". iApply ("Hcov" with "HΦ'").
+  Qed.
+
+  Lemma imp_sum η :
+    lookup_spec η ["Array"] (array_module_spec) -∗
+    lookup_spec η ["+"] (λ add, iSpec τ[Z;Z] add (λ i j m, imp m {{ λ n, ⌜(n = i + j)%Z⌝ }})) -∗
+    imp (eval η esum) {{ λ sum, □ iSpec τ[Z] sum sum_spec }}.
+  Proof.
+    iIntros "#Hmodule_spec #Hadd".
+    iApply imp_EAnon_pers.
+    iIntros "!>" (n Hpos).
+    iApply imp_please; iNext.
+    iApply (imp_ELet_var (B:=array)).
+    { iApply (imp_EApp_pers τ[Z;val]).
+      { iApply imp_EPath_spec.
+        rewrite lookup_spec_search; last reflexivity.
+        iApply (lookup_spec_step with "[$]").
+        iIntros (?) "#Harray_module".
+        unfold array_module_spec at 2. unfold context. simpl.
+        iDestruct "Harray_module" as "($ & _)". }
+      iApply imp_EPath_var; eauto.
+      iApply (imp_EAnon_pers τ[Z] (λ i m, imp m {{ λ j, ⌜(j = i + 1)%Z⌝ }})%I).
+      { iIntros (i) "!>". iApply imp_please; iNext.
+        iApply imp_EIntAdd. iApply imp_EPath_var; eauto. iApply imp_EInt.
+        iIntros "!>" (? j) "-> ->". auto. }
+      iIntros (f ?) "-> #Hf %m Hm".
+      iPoseProof (weaken_init_spec with "Hm") as "Hm".
+      iSpecialize ("Hm" $! Z _ _ Hpos).
+      iApply "Hm".
+      iIntros "!> !>".
+      iApply (iSpec_mono with "Hf"). iIntros (i m') "Hm Hbound".
+      iApply "Hm". }
+    iIntros (a) "(%xs & %Hlenxs & HownArr & #Hxs)".
+    iApply (imp_EApp_pers τ[val;Z;array]).
+    { iApply imp_EPath_spec.
+      rewrite lookup_spec_search; last reflexivity.
+      rewrite lookup_spec_search; last reflexivity.
+      iApply (lookup_spec_step with "[$]").
+      iIntros (?) "#Harray_module".
+      unfold array_module_spec at 2. unfold context. simpl.
+      iDestruct "Harray_module" as "(_ & _ & _ & Hfold_left & _)".
+      iApply (lookup_spec_mono with "Hfold_left").
+      iIntros "!>" (init) "Hinit". iApply "Hinit". }
+    { iApply imp_EPath_spec.
+      rewrite lookup_spec_search; last reflexivity.
+      rewrite lookup_spec_search; last reflexivity.
+      iAssumption. }
+    { iApply imp_EInt. }
+    { iApply imp_EPath_var; auto. }
+    iIntros (??) "-> %add #Hadd_ -> %m Hm".
+
+    unfold fold_left_spec, tapp.
+    iSpecialize ("Hm" $! Z _ _ _ xs (λ acc elems, let n := length elems in ⌜acc = n * (n + 1) / 2⌝)%I).
+    iApply (imp_mono_ret with "[-]").
+    iPoseProof (slice_of_own with "HownArr") as "(#Harr & Hslice)"; first reflexivity.
+    - iApply ("Hm" with "Harr Hslice").
+      { iIntros "!>".
+        iApply (iSpec_mono with "Hadd_").
+        iIntros (i j m') "Hm' %Hvisited %Hprefix %Hacc".
+        iApply (imp_mono_ret with "Hm'").
+        iIntros (? ->).
+        destruct Hprefix as (ys & ->).
+        iPoseProof (big_sepL_app with "Hxs") as "(Helems & Hys)".
+        iPoseProof (big_sepL_app with "Helems") as "(Hvisited & %Hj)".
+        specialize (Hj 0%nat j (list_lookup_singleton_eq_0 j)).
+        iPureIntro. length. rewrite Hacc Hj. rewrite /length.
+        generalize (Datatypes.length Hvisited).
+        intros n0. replace (n0 + 0)%nat with n0 by lia.
+        replace (n0 + 1 + 1) with (n0 + 2) by lia.
+        replace ((n0 + 1) * (n0 + 2)) with ((n0 + 1) * n0 + (n0 +1) * 2) by lia.
+        replace (((n0 + 1) * n0 + (n0 + 1) * 2) / 2) with (((n0 + 1) * n0) / 2 + (n0 + 1)).
+        rewrite Z.mul_comm. reflexivity.
+        by rewrite Z.div_add; last lia. }
+      { iPureIntro. length. rewrite Z.mul_0_l Zdiv_0_l. reflexivity. }
+    - iIntros "!>" (acc) "(%Hacc & Hslice)".
+      iPureIntro. rewrite Hacc Hlenxs. reflexivity.
+  Qed.
+
+End verification.
